$$
\begin{aligned}
\text{fpless}:& \tau_{0} = \text{\bf ref}(\_ \times \text{\bf lam}(\alpha_1, \alpha_2)(\alpha_3))\\
\text{lessa} :& \tau_{1} = \text{\bf ref}(\alpha_4) \\
\text{lessb} :& \tau_{2} = \text{\bf ref}(\alpha_5) \\
\text{res}   :& \tau_{3} = \text{\bf ref}(\alpha_6) = \text{\bf ref}(\bot \times \bot) \\
\text{less}  :& \tau_{4} = \text{\bf ref}(\_ \times \text{\bf lam}(\alpha_4, \alpha_5)(\alpha_6)) \\
			  & \alpha_{4} \unlhd \alpha_{1} \\
			  & \alpha_{5} \unlhd \alpha_{2} \\
			  & \alpha_{6} \unlhd \alpha_{3} \\



\text{v00}:   & \tau_{5} = \text{\bf ref}(\bot \times \bot) = \text{\bf ref}(\alpha_{7}) \\
\text{v01}:   & \tau_{6} = \text{\bf ref}(\bot \times \bot) = \text{\bf ref}(\alpha_{8}) \\
\text{A}     :& \tau_{10} = \text{\bf ref}(\text{\bf ref}(\_) \times \_) \\
\text{A}     :& \tau_{10} = \text{\bf ref}(\text{\bf ref}(\alpha_9) \times \_) \\
			  & \alpha_{7} \unlhd \alpha{9} \\



\text{B}     :& \tau_{11} = \text{\bf ref}(\alpha_{10}) \\
			  & \alpha_{8} \unlhd \alpha{10} \\
\text{A0}    :& \tau_{12} = \text{\bf ref}(\alpha_{11}) \\
			  & \alpha_{9} \unlhd \alpha{11} \\
\text{pA0}   :& \tau_{13} = \text{\bf ref}(\tau_{12} \times \_) \\
\text{pB}    :& \tau_{14} = \text{\bf ref}(\tau_{11} \times \_) \\


			  & \tau_{13} \unlhd \alpha_{4} \\
			  & \tau_{14} \unlhd \alpha_{5} \\
\text{g}     :& \tau_{15} = \text{\bf ref}(\bot \times \bot) \\


\text{pC}    :& \tau_{16} = \text{\bf ref}(\tau_{12} \times \_) \\
\text{pC}    :& \tau_{16} = \text{\bf ref}(\tau_{11} \times \_) \\
			  & \tau_{12} = \tau_{11} \\
			  & \alpha_{10} = \alpha_{11} \\


			  & \tau_{14} \unlhd \alpha_{4} \\
			  & \tau_{13} \unlhd \alpha_{5} \\
\text{g}     :& \tau_{15} = \text{\bf ref}(\bot \times \bot)

\end{aligned}
$$


$$
\begin{aligned} \text{v00}: & \tau_{5} = \text{\bf ref}(\bot \times \bot) = \text{\bf ref}(\alpha_{7}) \\ \text{v01}: & \tau_{6} = \text{\bf ref}(\bot \times \bot) = \text{\bf ref}(\alpha_{8}) \\ \text{A} :& \tau_{10} = \text{\bf ref}(\text{\bf ref}(\_) \times \_) \\ \text{A} :& \tau_{10} = \text{\bf ref}(\text{\bf ref}(\alpha_9) \times \_) \\ & \alpha_{7} \unlhd \alpha{9} \\ \text{B} :& \tau_{11} = \text{\bf ref}(\alpha_{10}) \\ & \alpha_{8} \unlhd \alpha{10} \\ \text{A0} :& \tau_{12} = \text{\bf ref}(\alpha_{11}) \\ & \alpha_{9} \unlhd \alpha{11} \\ \text{pA0} :& \tau_{13} = \text{\bf ref}(\tau_{12} \times \_) \\ \text{pB} :& \tau_{14} = \text{\bf ref}(\tau_{11} \times \_) \\ & \tau_{13} \unlhd \alpha_{4} \\ & \tau_{14} \unlhd \alpha_{5} \\ \text{g} :& \tau_{15} = \text{\bf ref}(\bot \times \bot) \\ \text{pC} :& \tau_{16} = \text{\bf ref}(\tau_{12} \times \_) \\ \text{pC} :& \tau_{16} = \text{\bf ref}(\tau_{11} \times \_) \\ & \tau_{12} = \tau_{11} \\ & \alpha_{10} = \alpha_{11} \\ & \tau_{14} \unlhd \alpha_{4} \\ & \tau_{13} \unlhd \alpha_{5} \\ \text{g} :& \tau_{15} = \text{\bf ref}(\bot \times \bot) \end{aligned}
$$